By utilizing

.. math::

    2 \cos \alpha
    =
    \frac{
        \cos \left( \alpha + \beta \right)
        +
        \cos \left( \alpha - \beta \right)
    }{\cos \beta}

with

.. math::

    \beta
    &
    =
    \beta \left( n \right)
    =
    2
    \pi
    \frac{n + \frac{1}{2}}{2 N},

    \alpha
    &
    =
    \alpha \left( n, k \right)
    =
    \beta
    \left( 2 k + 1 \right),

we obtain

.. math::

    &
    2
    \sum_{k = 0}^{N / 2 - 1}
    X_{2 k + 1}
    \ctwiddle{2 \pi}{\left( n + \frac{1}{2} \right) \left( 2 k + 1 \right)}{2 N}

    =
    &
    2
    \sum_{k = 0}^{N / 2 - 1}
    X_{2 k + 1}
    \cos \alpha

    =
    &
    \frac{1}{\cos \beta}
    \sum_{k = 0}^{N / 2 - 1}
    X_{2 k + 1}
    \left[
        \cos \left( \alpha + \beta \right)
        +
        \cos \left( \alpha - \beta \right)
    \right]

    =
    &
    \frac{1}{\cos \beta}
    \sum_{k = 0}^{N / 2 - 1}
    X_{2 k + 1}
    \ctwiddle{2 \pi}{\left( n + \frac{1}{2} \right) \left( 2 k + 2 \right)}{2 N}
    +
    \frac{1}{\cos \beta}
    \sum_{k = 0}^{N / 2 - 1}
    X_{2 k + 1}
    \ctwiddle{2 \pi}{\left( n + \frac{1}{2} \right) \left( 2 k     \right)}{2 N}

    =
    &
    \frac{1}{\cos \beta}
    \sum_{l = 1}^{N / 2}
    X_{2 l - 1}
    \ctwiddle{2 \pi}{\left( n + \frac{1}{2} \right) \left( 2 l \right)}{2 N}
    +
    \frac{1}{\cos \beta}
    \sum_{k = 0}^{N / 2 - 1}
    X_{2 k + 1}
    \ctwiddle{2 \pi}{\left( n + \frac{1}{2} \right) \left( 2 k \right)}{2 N}

    =
    &
    \frac{1}{\cos \beta}
    \sum_{k = 1}^{N / 2}
    X_{2 k - 1}
    \ctwiddle{2 \pi}{\left( n + \frac{1}{2} \right) \left( 2 k \right)}{2 N}
    +
    \frac{1}{\cos \beta}
    \sum_{k = 0}^{N / 2 - 1}
    X_{2 k + 1}
    \ctwiddle{2 \pi}{\left( n + \frac{1}{2} \right) \left( 2 k \right)}{2 N}.

